src/spec/Flutterbye.Seq.ToSet.fst
@@ -1,0 +1,61 @@
+// $legal:629:
+//
+// Copyright 2016 Michael Lowell Roberts & Microsoft Research
+//
+// Licensed under the Apache License, Version 2.0 (the "License");
+// you may not use this file except in compliance with the License.
+// You may obtain a copy of the License at
+//
+//     http://www.apache.org/licenses/LICENSE-2.0
+//
+// Unless required by applicable law or agreed to in writing, software
+// distributed under the License is distributed on an "AS IS" BASIS,
+// WITHOUT WARRANTIES OR CONDITIONS OF ANY KIND, either express or implied.
+// See the License for the specific language governing permissions and
+// limitations under the License.
+//
+//,$
+
+module Flutterbye.Seq.ToSet
+open FStar.Seq
+open FStar.Set
+
+private val to_set_loop:
+   s:seq 'a ->
+   i:nat{i <= length s} ->
+   ac:set 'a ->
+   Tot (set 'a)
+      (decreases (length s - i))
+let rec to_set_loop s i ac =
+   if i < length s then
+      let a = index s i in
+      let ac' = union ac (singleton a) in
+      to_set_loop s (i + 1) ac'
+   else
+      ac
+
+private type from_seq_p (#a:Type) (s:seq a) (s':set a) =
+   (length s = 0 /\ FStar.Set.equal s' FStar.Set.empty) \/
+   (forall x.
+      Flutterbye.Seq.Mem.mem_p x s <==> b2t (mem x s'))
+
+private val to_set_lemma:
+   s:seq 'a ->
+   i:nat{i <= length s} ->
+   ac:set 'a ->
+   Lemma
+      (requires (from_seq_p (slice s 0 i) ac))
+      (ensures (from_seq_p s (to_set_loop s i ac)))
+      (decreases (length s - i))
+let rec to_set_lemma s i ac =
+   if i < length s then
+      let a = index s i in
+      let ac' = union ac (singleton a) in
+      to_set_lemma s (i + 1) ac'
+   else
+      ()
+
+val to_set: (s:seq 'a) -> Tot (s':set 'a{from_seq_p s s'})
+let to_set s =
+   to_set_lemma s 0 empty;
+   to_set_loop s 0 empty
